Update SkipList.Remove.fst

SkipList2/SkipList.Remove.fst
@@ -71,12 +71,26 @@ let rebuildIndexes #a #f sl place =
         let seq_replace = Seq.create (Sl.length sl - 1) [0] in 
         rebuildIndexesSeq #a #f sl place seq_replace 0 
 
- val rebuildSequence: #a: eqtype ->  #f: cmp a -> s:seq a{Seq.sorted f s /\ Seq.length s > 1 } ->  
-                place: nat {place < Seq.length s - 1} ->
-                Tot (r: seq a {Seq.sorted f r /\ Seq.length r = Seq.length s - 1})
-
-assume val concat: #a: eqtype ->#f: cmp a ->  s1 : seq a {Seq.sorted f s1 } -> s2: seq a {Seq.sorted f s2} -> 
+val concat: #a: eqtype ->#f: cmp a ->  s1 : seq a {Seq.sorted f s1 } -> s2: seq a {Seq.sorted f s2 /\
+(Seq.length s1 > 0 /\ Seq.length s2 > 0 /\ f (seqLast s1) (seqFirst s2))} -> 
     Tot(s3: seq a {Seq.sorted f s3 /\ Seq.length s3 = Seq.length s1 + Seq.length s2})
+
+let concat #a #f s1 s2 = 
+        let pivot = seqFirst s2 in 
+        let seq2 = Seq.tail s2 in 
+        assert(f (seqLast s1) pivot);
+        if (Seq.length seq2 = 0 ) then 
+            ordered_addition_l #a #f pivot s1
+        else (
+            tail_mem_left_wrapper #a #f pivot seq2; 
+            assert(forall y. (Seq.mem y seq2 ==> f pivot y));
+            assert(Seq.sorted f seq2);
+            tail_mem #a #f pivot s1; 
+            assert(forall y. (Seq.mem y s1 ==> f y pivot));
+            let r = sorted_seq_concat_wrapper #a #f pivot s1 seq2 
+            in r
+        )
+
 
 assume val lemma_split: #a : eqtype -> #f: cmp a-> 
             s: seq a {Seq.length s > 0 /\ Seq.sorted f s} ->
@@ -87,17 +101,29 @@ assume val lemma_split: #a : eqtype -> #f: cmp a->
                                         (Seq.sorted f (snd(Seq.split s place)))
                                 ))
 
+assume val lemma_sorted : #a: eqtype -> #f : cmp a -> s: seq a {Seq.sorted f s} ->
+            place : nat {place > 0 /\ place < Seq.length s -1 } -> 
+            Lemma (ensures (f (Seq.index s (place -1)) (Seq.index s place)))
+
+val rebuildSequence: #a: eqtype ->  #f: cmp a -> s:seq a{Seq.sorted f s /\ Seq.length s > 1 } ->  
+                place: nat {place < Seq.length s - 1} ->
+                Tot (r: seq a {Seq.sorted f r /\ Seq.length r = Seq.length s - 1})
+
+
 let rebuildSequence #a #f s place = 
-    let s1, s2 = Seq.split s place in 
-    assert(Seq.length s1 + Seq.length s2 = Seq.length s);
+    let s1, s2 = Seq.split s place in (*place < Seq.length s -1  - it means that there is at least ONE element in right seq*)
     lemma_split #a #f s place;
-    let s3, s4 = Seq.split s2 1 in 
-    assert(Seq.length s4 = Seq.length s - Seq.length s1 -1);
+    let s3, s4 = Seq.split s2 1 in(* s3 has one element, while s4 could not have any*)
     lemma_split #a #f s2 1;
-    assert (Seq.sorted f s4);
-    assert(Seq.sorted f s1);
-    let r = concat #a #f s1 s4    
-    in r            
+    if Seq.length s1 = 0 then s4
+    else if (Seq.length s4 = 0) then s1
+    else
+        (
+            lemma_sorted #a #f s place; 
+            assert(f (Seq.index s (place -1)) (Seq.index s (place)));
+            assert(f (seqLast s1) (seqFirst s4));    
+            concat #a #f s1 s4
+        )        
 
 val remove: #a: eqtype -> #f : cmp a -> 
         sl: skipList a f {Sl.length sl > 1} -> 
@@ -109,4 +135,4 @@ let remove #a #f sl place =
     let indexes = Sl.getIndexes sl in 
     let values_new = rebuildSequence #a #f values place in 
     let indexes_new = rebuildIndexes #a #f sl place in 
-    Sl.Mk #a #f values_new indexes_new       
+    Sl.Mk #a #f values_new indexes_new 
